Replace `AST.rettype` by `AST.xtype`
- `AST.xtype` is not built on top of `AST.type`, but has its own constructors.
- Added a `Xptr` case, to be used for ABIs that pass pointers and integers
  in different register classes.

backend/PrintAsmaux.ml
@@ -100,7 +100,7 @@ let reset_literals () =
 
 let current_function_stacksize = ref 0l
 let current_function_sig =
-  ref { sig_args = []; sig_res = Tvoid; sig_cc = cc_default }
+  ref { sig_args = []; sig_res = Xvoid; sig_cc = cc_default }
 
 (* Functions for printing of symbol names *)
 let elf_symbol oc symb =
@@ -269,8 +269,8 @@ let re_asm_param_2 = Str.regexp "%\\([QR]?\\)\\([0-9]+\\)"
 let print_inline_asm print_preg oc txt sg args res =
   let (operands, ty_operands) =
     match sg.sig_res with
-    | Tvoid -> (args, proj_sig_args sg)
-    | tres -> (builtin_arg_of_res res :: args, proj_rettype tres :: proj_sig_args sg) in
+    | Xvoid -> (args, proj_sig_args sg)
+    | tres -> (builtin_arg_of_res res :: args, proj_xtype tres :: proj_sig_args sg) in
   let print_fragment = function
   | Str.Text s ->
       output_string oc s
