x86/Asmexpand.ml
@@ -536,7 +536,7 @@ let expand_instruction instr =
        if is_current_function_variadic() then
          (* Save parameters passed in registers in reserved stack area *)
          emit (Pcall_s (intern_string "__compcert_va_saveregs",
-                        {sig_args = []; sig_res = Tvoid; sig_cc = cc_default}));
+                        {sig_args = []; sig_res = Xvoid; sig_cc = cc_default}));
        (* Allocate frame *)
        let sz' = Z.of_uint sz in
        emit (Psubq_ri (RSP, sz'));
@@ -557,7 +557,7 @@ let expand_instruction instr =
          (* Save the registers *)
          emit_leaq R10 (linear_addr RSP (Z.of_uint save_regs));
          emit (Pcall_s (intern_string "__compcert_va_saveregs",
-                        {sig_args = []; sig_res = Tvoid; sig_cc = cc_default}))
+                        {sig_args = []; sig_res = Xvoid; sig_cc = cc_default}))
        end;
        (* Stack chaining *)
        let fullsz = sz + 8 in
