backend/RTLgenspec.v
@@ -640,7 +640,7 @@ Lemma new_reg_return_ok:
   return_reg_ok s2 map (ret_reg sig r).
 Proof.
   intros. unfold ret_reg.
-  destruct (rettype_eq (sig_res sig) Tvoid); constructor; eauto with rtlg.
+  destruct (xtype_eq (sig_res sig) Xvoid); constructor; eauto with rtlg.
 Qed.
 
 (** * Relational specification of the translation *)
@@ -1224,7 +1224,7 @@ Lemma convert_builtin_res_charact:
 Proof.
   destruct res; simpl; intros.
 - monadInv TR. constructor.  unfold find_var in EQ. destruct (map_vars map)!x; inv EQ; auto.
-- destruct (rettype_eq oty Tvoid); monadInv TR.
+- destruct (xtype_eq oty Xvoid); monadInv TR.
 + constructor.
 + constructor. eauto with rtlg.
 - monadInv TR.
@@ -1348,7 +1348,7 @@ Proof.
   intros [C D].
   eapply tr_function_intro; eauto with rtlg.
   eapply transl_stmt_charact; eauto with rtlg.
-  unfold ret_reg. destruct (rettype_eq (sig_res (CminorSel.fn_sig f)) Tvoid).
+  unfold ret_reg. destruct (xtype_eq (sig_res (CminorSel.fn_sig f)) Xvoid).
   constructor.
   constructor; eauto with rtlg.
 Qed.
