backend/RTLtyping.v
@@ -151,11 +151,11 @@ Inductive wt_instr : instruction -> Prop :=
       list_length_z tbl * 4 <= Int.max_unsigned ->
       wt_instr (Ijumptable arg tbl)
   | wt_Ireturn_none:
-      funct.(fn_sig).(sig_res) = Tvoid ->
+      funct.(fn_sig).(sig_res) = Xvoid ->
       wt_instr (Ireturn None)
   | wt_Ireturn_some:
       forall arg ty,
-      funct.(fn_sig).(sig_res) <> Tvoid ->
+      funct.(fn_sig).(sig_res) <> Xvoid ->
       env arg = proj_sig_res funct.(fn_sig) ->
       env arg = ty ->
       wt_instr (Ireturn (Some arg)).
@@ -299,7 +299,7 @@ Definition type_instr (e: S.typenv) (i: instruction) : res S.typenv :=
   | Itailcall sig ros args =>
       do e1 <- type_ros e ros;
       do e2 <- S.set_list e1 args (proj_sig_args sig);
-      if rettype_eq sig.(sig_res) f.(fn_sig).(sig_res) then
+      if xtype_eq sig.(sig_res) f.(fn_sig).(sig_res) then
         if tailcall_is_possible sig
         then OK e2
         else Error(msg "tailcall not possible")
@@ -324,7 +324,7 @@ Definition type_instr (e: S.typenv) (i: instruction) : res S.typenv :=
       then OK e1
       else Error(msg "jumptable too big")
   | Ireturn optres =>
-      match optres, rettype_eq f.(fn_sig).(sig_res) Tvoid with
+      match optres, xtype_eq f.(fn_sig).(sig_res) Xvoid with
       | None, left _ => OK e
       | Some r, right _ => S.set e r (proj_sig_res f.(fn_sig))
       | _, _ => Error(msg "bad return")
@@ -469,7 +469,7 @@ Proof.
   destruct l; try discriminate. destruct l; monadInv EQ0. eauto with ty.
   destruct (type_of_operation o) as [targs tres] eqn:TYOP. monadInv EQ0. eauto with ty.
 - (* tailcall *)
-  destruct (rettype_eq (sig_res s) (sig_res (fn_sig f))); try discriminate.
+  destruct (xtype_eq (sig_res s) (sig_res (fn_sig f))); try discriminate.
   destruct (tailcall_is_possible s) eqn:TCIP; inv EQ2.
   eauto with ty.
 - (* builtin *)
@@ -479,7 +479,7 @@ Proof.
   eauto with ty.
 - (* return *)
   simpl in H.
-  destruct o as [r|] eqn: RET; destruct (rettype_eq (sig_res (fn_sig f)) Tvoid); try discriminate.
+  destruct o as [r|] eqn: RET; destruct (xtype_eq (sig_res (fn_sig f)) Xvoid); try discriminate.
   eauto with ty.
   inv H; auto with ty.
 Qed.
@@ -521,7 +521,7 @@ Proof.
   eapply S.set_sound; eauto with ty.
   eauto with ty.
 - (* tailcall *)
-  destruct (rettype_eq (sig_res s) (sig_res (fn_sig f))); try discriminate.
+  destruct (xtype_eq (sig_res s) (sig_res (fn_sig f))); try discriminate.
   destruct (tailcall_is_possible s) eqn:TCIP; inv EQ2.
   constructor.
   eapply type_ros_sound; eauto with ty.
@@ -546,7 +546,7 @@ Proof.
   auto.
 - (* return *)
   simpl in H.
-  destruct o as [r|] eqn: RET; destruct (rettype_eq (sig_res (fn_sig f)) Tvoid); try discriminate.
+  destruct o as [r|] eqn: RET; destruct (xtype_eq (sig_res (fn_sig f)) Xvoid); try discriminate.
   econstructor. auto. eapply S.set_sound; eauto with ty. eauto.
   inv H. constructor. auto.
 Qed.
@@ -875,7 +875,7 @@ Qed.
 
 Inductive wt_stackframes: list stackframe -> signature -> Prop :=
   | wt_stackframes_nil: forall sg,
-      sg.(sig_res) = Tint ->
+      sg.(sig_res) = Xint ->
       wt_stackframes nil sg
   | wt_stackframes_cons:
       forall s res f sp pc rs env sg,
