cfrontend/Cop.v
@@ -1645,12 +1645,9 @@ Qed.
 Lemma val_casted_has_argtype:
   forall v ty, val_casted v ty -> Val.has_argtype v (argtype_of_type ty).
 Proof.
-  destruct 1; simpl; unfold Tptr; rewrite ? H; auto.
+  destruct 1; simpl; rewrite ? H; auto.
 - destruct sz; [destruct si | destruct si | | ]; simpl in *; auto.
   destruct (Int.eq n Int.zero); auto.
-- destruct Archi.ptr64; auto.
-- destruct Archi.ptr64; auto.
-- destruct Archi.ptr64; auto.
 Qed.
 
 (** Likewise, casted values belong to the machine type corresponding to the
